Setting ep to false when the basicblock has a header. MBgoto done. MBgetparam needs fix

mppa_k1c/Asmblockgen.v
@@ -903,13 +903,11 @@ Fixpoint transl_blocks (f: Machblock.function) (lmb: list Machblock.bblock) (ep:
   match lmb with
   | nil => OK nil
   | mb :: lmb => 
-      do lb <- transl_block f mb ep;
+      do lb <- transl_block f mb (if Machblock.header mb then ep else false);
       do lb' <- transl_blocks f lmb false;
       OK (lb ++ lb')
   end
 .
-
-
 
 Definition transl_function (f: Machblock.function) :=
   do lb <- transl_blocks f f.(Machblock.fn_code) true;
